start clarification of when a program fails
This developments tries to make it more explicit when a bir program
returns the status code "BST_Failed". However, before this real goal can
be even started, some infrastructure about the variables used by a
program is needed. This commit introduces the variables used (read and
written) and changed (written) by statements, blocks and programs. It is
then shown that a program at most changes the vars in its read-set and
the execution depends only on the vars in the whole set.

This should provide the background to formally talk about the failed
status.

src/core-props/bir_program_blocksScript.sml
@@ -489,7 +489,7 @@ ASM_SIMP_TAC list_ss [rich_listTheory.SEG_LENGTH_ID]);
 val bir_block_size_def = Define `bir_block_size bl = SUC (LENGTH bl.bb_statements)`;
 
 
-val bir_exec_block_def = Define `bir_exec_block p bl st =
+val bir_exec_block_def = Define `bir_exec_block (p:'a bir_program_t) (bl:'a bir_block_t) st =
   let (l, c, st') = bir_exec_stmtsB bl.bb_statements ([], 0, st) in
   (if (bir_state_is_terminated st') then
     (l, c, st' with bst_pc := (st.bst_pc with bpc_index := st.bst_pc.bpc_index + PRE c))
