src/core/bir_typing_progScript.sml
@@ -3,13 +3,47 @@ open wordsTheory bitstringTheory;
 open bir_auxiliaryTheory bir_immTheory bir_valuesTheory;
 open bir_imm_expTheory bir_mem_expTheory bir_envTheory;
 open bir_expTheory bir_typing_expTheory bir_programTheory;
-open wordsLib;
+open wordsLib pred_setTheory;
 
 val _ = new_theory "bir_typing_prog";
 
 
 (* ------------------------------------------------------------------------- *)
-(*  Programs                                                                 *)
+(*  Statements of Programs                                                   *)
+(* ------------------------------------------------------------------------- *)
+
+val bir_stmts_of_block_def = Define `bir_stmts_of_block bl =
+  (BStmtE (bl.bb_last_statement) INSERT (IMAGE BStmtB (set bl.bb_statements)))`;
+
+val bir_stmts_of_prog_def = Define `bir_stmts_of_prog (BirProgram p) =
+  BIGUNION (IMAGE bir_stmts_of_block (set p))`;
+
+val bir_get_current_statement_stmts_of_prog = store_thm ("bir_get_current_statement_stmts_of_prog",
+  ``!p pc stmt. (bir_get_current_statement p pc = SOME stmt) ==>
+                stmt IN (bir_stmts_of_prog p)``,
+
+Cases >> rename1 `BirProgram p` >>
+SIMP_TAC std_ss [bir_get_current_statement_def, bir_stmts_of_prog_def,
+  IN_BIGUNION, IN_IMAGE, PULL_EXISTS, bir_stmts_of_block_def,
+  IN_INSERT, IN_IMAGE] >>
+REPEAT GEN_TAC >>
+Cases_on `(bir_get_program_block_info_by_label (BirProgram p) pc.bpc_label)` >- (
+  ASM_SIMP_TAC std_ss []
+) >>
+rename1 `_ = SOME xy` >> Cases_on `xy` >>
+rename1 `_ = SOME (i, bl)` >>
+ASM_SIMP_TAC (std_ss++boolSimps.LIFT_COND_ss) [] >>
+CASE_TAC >> STRIP_TAC >> REPEAT BasicProvers.VAR_EQ_TAC >> (
+  FULL_SIMP_TAC std_ss [bir_get_program_block_info_by_label_THM,
+    bir_stmt_t_11, bir_stmt_t_distinct] >>
+  METIS_TAC[rich_listTheory.EL_MEM]
+));
+
+
+
+
+(* ------------------------------------------------------------------------- *)
+(*  Well-typed Programs                                                      *)
 (* ------------------------------------------------------------------------- *)
 
 val bir_is_well_typed_label_exp_def = Define `
@@ -20,7 +54,7 @@ val bir_is_well_typed_label_exp_def = Define `
 
 val bir_is_well_typed_stmtE_def = Define `
   (bir_is_well_typed_stmtE (BStmt_Jmp le) = bir_is_well_typed_label_exp le) /\
-  (bir_is_well_typed_stmtE (BStmt_CJmp c le1 le2) = 
+  (bir_is_well_typed_stmtE (BStmt_CJmp c le1 le2) =
        (type_of_bir_exp c = SOME BType_Bool) /\
        (bir_is_well_typed_label_exp le1) /\
        (bir_is_well_typed_label_exp le2)) /\
@@ -38,36 +72,197 @@ val bir_is_well_typed_stmt_def = Define `
   (bir_is_well_typed_stmt (BStmtB s) = bir_is_well_typed_stmtB s)`;
 
 val bir_is_well_typed_block_def = Define `bir_is_well_typed_block bl <=>
-  ((EVERY bir_is_well_typed_stmtB bl.bb_statements) /\ 
+  ((EVERY bir_is_well_typed_stmtB bl.bb_statements) /\
    (bir_is_well_typed_stmtE bl.bb_last_statement))`;
 
 val bir_is_well_typed_program_def = Define `bir_is_well_typed_program (BirProgram p) <=>
   (EVERY bir_is_well_typed_block p)`;
+
+val bir_is_well_typed_block_ALT_DEF = store_thm ("bir_is_well_typed_block_ALT_DEF",
+  ``!bl. bir_is_well_typed_block bl <=>
+    (!stmt. stmt IN bir_stmts_of_block bl ==> bir_is_well_typed_stmt stmt)``,
+
+SIMP_TAC (std_ss++boolSimps.EQUIV_EXTRACT_ss) [bir_is_well_typed_block_def, bir_stmts_of_block_def,
+  IN_INSERT, IN_IMAGE, DISJ_IMP_THM, PULL_EXISTS, FORALL_AND_THM,
+  bir_is_well_typed_stmt_def, listTheory.EVERY_MEM]);
+
+val bir_is_well_typed_program_ALT_DEF = store_thm ("bir_is_well_typed_program_ALT_DEF",
+  ``!p. bir_is_well_typed_program p <=>
+    (!stmt. stmt IN bir_stmts_of_prog p ==> bir_is_well_typed_stmt stmt)``,
+
+Cases >>
+SIMP_TAC std_ss [bir_is_well_typed_program_def,
+  bir_stmts_of_prog_def, IN_BIGUNION, IN_IMAGE, PULL_EXISTS,
+  listTheory.EVERY_MEM, bir_is_well_typed_block_ALT_DEF] >>
+METIS_TAC[]);
 
 
 val bir_get_current_statement_well_typed = store_thm ("bir_get_current_statement_well_typed",
   ``!p pc stmt. (bir_is_well_typed_program p /\
                 (bir_get_current_statement p pc = SOME stmt)) ==>
                 bir_is_well_typed_stmt stmt``,
+METIS_TAC[bir_is_well_typed_program_ALT_DEF, bir_get_current_statement_stmts_of_prog]);
 
-Cases >> rename1 `BirProgram p` >>
-SIMP_TAC std_ss [bir_is_well_typed_program_def, bir_get_current_statement_def] >>
-GEN_TAC >>
-Cases_on `(bir_get_program_block_info_by_label (BirProgram p) pc.bpc_label)` >- (
-  ASM_SIMP_TAC std_ss []
+
+
+
+(* ------------------------------------------------------------------------- *)
+(*  Variables of statements and programs                                     *)
+(* ------------------------------------------------------------------------- *)
+
+val bir_vars_of_stmtB_def = Define `
+  (bir_vars_of_stmtB (BStmt_Declare v) = {v}) /\
+  (bir_vars_of_stmtB (BStmt_Assert ex) = bir_vars_of_exp ex) /\
+  (bir_vars_of_stmtB (BStmt_Assume ex) = bir_vars_of_exp ex) /\
+  (bir_vars_of_stmtB (BStmt_Assign v ex) = (v INSERT (bir_vars_of_exp ex))) /\
+  (bir_vars_of_stmtB (BStmt_Observe ec el obf) =
+     BIGUNION (IMAGE bir_vars_of_exp (LIST_TO_SET (ec::el))))`;
+
+val bir_vars_of_label_exp_def = Define `
+  (bir_vars_of_label_exp (BLE_Label l) = {}) /\
+  (bir_vars_of_label_exp (BLE_Exp e) = bir_vars_of_exp e)`;
+
+val bir_vars_of_stmtE_def = Define `
+  (bir_vars_of_stmtE (BStmt_Jmp l) = bir_vars_of_label_exp l) /\
+  (bir_vars_of_stmtE (BStmt_CJmp e l1 l2) =
+    (bir_vars_of_exp e UNION (bir_vars_of_label_exp l1) UNION (bir_vars_of_label_exp l2))) /\
+  (bir_vars_of_stmtE (BStmt_Halt ex) = bir_vars_of_exp ex)`;
+
+val bir_vars_of_stmt_def = Define `
+  (bir_vars_of_stmt (BStmtE s) = bir_vars_of_stmtE s) /\
+  (bir_vars_of_stmt (BStmtB s) = bir_vars_of_stmtB s)`;
+
+val bir_vars_of_block_def = Define `bir_vars_of_block bl <=>
+  ((BIGUNION (IMAGE bir_vars_of_stmtB (LIST_TO_SET bl.bb_statements))) UNION
+   (bir_vars_of_stmtE bl.bb_last_statement))`;
+
+val bir_vars_of_program_def = Define `bir_vars_of_program (BirProgram p) <=>
+  (BIGUNION (IMAGE bir_vars_of_block (LIST_TO_SET p)))`;
+
+val bir_vars_of_block_ALT_DEF = store_thm ("bir_vars_of_block_ALT_DEF",
+  ``!bl. bir_vars_of_block bl = BIGUNION (IMAGE bir_vars_of_stmt (bir_stmts_of_block bl))``,
+
+SIMP_TAC std_ss [EXTENSION] >>
+SIMP_TAC (std_ss++boolSimps.EQUIV_EXTRACT_ss) [bir_vars_of_block_def, bir_stmts_of_block_def,
+  IN_BIGUNION, PULL_EXISTS, IN_UNION, bir_vars_of_stmt_def,
+  IN_IMAGE, IN_INSERT, LEFT_AND_OVER_OR, EXISTS_OR_THM]);
+
+
+val bir_vars_of_program_ALT_DEF = store_thm ("bir_vars_of_program_ALT_DEF",
+  ``!p. bir_vars_of_program p =
+        BIGUNION (IMAGE bir_vars_of_stmt (bir_stmts_of_prog p))``,
+
+Cases >>
+SIMP_TAC std_ss [EXTENSION] >>
+SIMP_TAC std_ss [bir_vars_of_program_def, bir_stmts_of_prog_def,
+  IN_BIGUNION, PULL_EXISTS, IN_IMAGE, bir_vars_of_block_ALT_DEF] >>
+METIS_TAC[]);
+
+
+val bir_get_current_statement_vars_of = store_thm ("bir_get_current_statement_vars_of",
+  ``!p pc stmt. (bir_get_current_statement p pc = SOME stmt) ==>
+                bir_vars_of_stmt stmt SUBSET bir_vars_of_program p``,
+
+SIMP_TAC std_ss [bir_vars_of_program_ALT_DEF, SUBSET_DEF, IN_BIGUNION,
+  IN_IMAGE, PULL_EXISTS] >>
+METIS_TAC[bir_get_current_statement_stmts_of_prog]);
+
+
+val bir_vars_of_label_exp_THM_EQ_FOR_VARS = store_thm ("bir_vars_of_label_exp_THM_EQ_FOR_VARS",
+``!env1 env2 e. (bir_env_EQ_FOR_VARS (bir_vars_of_label_exp e) env1 env2) ==>
+                (bir_eval_label_exp e env1 = bir_eval_label_exp e env2)``,
+Cases_on `e` >> (
+  SIMP_TAC std_ss [bir_eval_label_exp_def, bir_vars_of_label_exp_def]
 ) >>
-rename1 `_ = SOME xy` >> Cases_on `xy` >>
-rename1 `_ = SOME (i, bl)` >>
-ASM_SIMP_TAC (std_ss++boolSimps.LIFT_COND_ss) [] >>
-Cases_on `EVERY bir_is_well_typed_block p` >> ASM_SIMP_TAC std_ss [] >>
-`bir_is_well_typed_block bl` by (
-  `MEM bl p` by METIS_TAC [bir_get_program_block_info_by_label_THM, listTheory.MEM_EL] >>
-  METIS_TAC[listTheory.EVERY_MEM]
-) >>
-CASE_TAC >> (
-  FULL_SIMP_TAC std_ss [bir_is_well_typed_block_def, bir_is_well_typed_stmt_def]
-) >>
-METIS_TAC[listTheory.EVERY_MEM, listTheory.MEM_EL]);
+METIS_TAC[bir_vars_of_exp_THM_EQ_FOR_VARS]);
+
+
+
+(* ------------------------------- *)
+(*  Variables modified by program  *)
+(* ------------------------------- *)
+
+
+val bir_changed_vars_of_stmtB_def = Define `
+  (bir_changed_vars_of_stmtB (BStmt_Declare v) = {v}) /\
+  (bir_changed_vars_of_stmtB (BStmt_Assert ex) = {}) /\
+  (bir_changed_vars_of_stmtB (BStmt_Assume ex) = {}) /\
+  (bir_changed_vars_of_stmtB (BStmt_Assign v ex) = {v}) /\
+  (bir_changed_vars_of_stmtB (BStmt_Observe ec el obf) = {})`;
+
+val bir_changed_vars_of_stmt_def = Define `
+  (bir_changed_vars_of_stmt (BStmtE s) = {}) /\
+  (bir_changed_vars_of_stmt (BStmtB s) = bir_changed_vars_of_stmtB s)`;
+
+val bir_changed_vars_of_block_def = Define `bir_changed_vars_of_block bl <=>
+  (BIGUNION (IMAGE bir_changed_vars_of_stmtB (LIST_TO_SET bl.bb_statements)))`;
+
+val bir_changed_vars_of_program_def = Define `bir_changed_vars_of_program (BirProgram p) <=>
+  (BIGUNION (IMAGE bir_changed_vars_of_block (LIST_TO_SET p)))`;
+
+val bir_changed_vars_of_stmtB_SUBST_all_vars = store_thm (
+  "bir_changed_vars_of_stmtB_SUBST_all_vars",
+``!stmt. bir_changed_vars_of_stmtB stmt SUBSET bir_vars_of_stmtB stmt``,
+Cases >> (
+  SIMP_TAC std_ss [bir_vars_of_stmtB_def, bir_changed_vars_of_stmtB_def,
+    SUBSET_DEF, NOT_IN_EMPTY, IN_INSERT]
+));
+
+
+val bir_changed_vars_of_stmt_SUBST_all_vars = store_thm (
+  "bir_changed_vars_of_stmt_SUBST_all_vars",
+``!stmt. bir_changed_vars_of_stmt stmt SUBSET bir_vars_of_stmt stmt``,
+Cases >> (
+   SIMP_TAC std_ss [bir_changed_vars_of_stmt_def, bir_vars_of_stmt_def,
+     bir_changed_vars_of_stmtB_SUBST_all_vars, EMPTY_SUBSET]
+));
+
+
+val bir_changed_vars_of_block_SUBST_all_vars = store_thm (
+  "bir_changed_vars_of_block_SUBST_all_vars",
+``!bl. bir_changed_vars_of_block bl SUBSET bir_vars_of_block bl``,
+
+SIMP_TAC std_ss [bir_changed_vars_of_block_def, bir_vars_of_block_def,
+  SUBSET_DEF, IN_UNION, IN_BIGUNION, IN_IMAGE, PULL_EXISTS] >>
+METIS_TAC[SUBSET_DEF, bir_changed_vars_of_stmtB_SUBST_all_vars]);
+
+val bir_changed_vars_of_program_SUBST_all_vars = store_thm (
+  "bir_changed_vars_of_program_SUBST_all_vars",
+``!p. bir_changed_vars_of_program p SUBSET bir_vars_of_program p``,
+
+Cases >>
+SIMP_TAC std_ss [bir_changed_vars_of_program_def, bir_vars_of_program_def,
+  SUBSET_DEF, IN_UNION, IN_BIGUNION, IN_IMAGE, PULL_EXISTS] >>
+METIS_TAC[SUBSET_DEF, bir_changed_vars_of_block_SUBST_all_vars]);
+
+
+val bir_changed_vars_of_block_ALT_DEF = store_thm ("bir_changed_vars_of_block_ALT_DEF",
+  ``!bl. bir_changed_vars_of_block bl = BIGUNION (IMAGE bir_changed_vars_of_stmt (bir_stmts_of_block bl))``,
+
+SIMP_TAC std_ss [EXTENSION] >>
+SIMP_TAC (std_ss++boolSimps.EQUIV_EXTRACT_ss) [bir_changed_vars_of_block_def, bir_stmts_of_block_def,
+  IN_BIGUNION, PULL_EXISTS, IN_UNION, bir_changed_vars_of_stmt_def,
+  IN_IMAGE, IN_INSERT, LEFT_AND_OVER_OR, EXISTS_OR_THM, NOT_IN_EMPTY]);
+
+
+val bir_changed_vars_of_program_ALT_DEF = store_thm ("bir_changed_vars_of_program_ALT_DEF",
+  ``!p. bir_changed_vars_of_program p =
+        BIGUNION (IMAGE bir_changed_vars_of_stmt (bir_stmts_of_prog p))``,
+
+Cases >>
+SIMP_TAC std_ss [EXTENSION] >>
+SIMP_TAC std_ss [bir_changed_vars_of_program_def, bir_stmts_of_prog_def,
+  IN_BIGUNION, PULL_EXISTS, IN_IMAGE, bir_changed_vars_of_block_ALT_DEF] >>
+METIS_TAC[]);
+
+
+val bir_get_current_statement_changed_vars_of = store_thm ("bir_get_current_statement_changed_vars_of",
+  ``!p pc stmt. (bir_get_current_statement p pc = SOME stmt) ==>
+                bir_changed_vars_of_stmt stmt SUBSET bir_changed_vars_of_program p``,
+
+SIMP_TAC std_ss [bir_changed_vars_of_program_ALT_DEF, SUBSET_DEF, IN_BIGUNION,
+  IN_IMAGE, PULL_EXISTS] >>
+METIS_TAC[bir_get_current_statement_stmts_of_prog]);
 
 
 val _ = export_theory();
