src/core-props/bir_program_varsScript.sml
@@ -1,0 +1,664 @@
+open HolKernel Parse boolLib bossLib;
+open bir_envTheory bir_valuesTheory
+open bir_programTheory HolBACoreSimps;
+open bir_program_multistep_propsTheory;
+open bir_program_env_orderTheory;
+open bir_typing_progTheory;
+open bir_program_blocksTheory
+open bir_typing_expTheory
+open pred_setTheory;
+
+val _ = new_theory "bir_program_vars";
+
+(* This theory shows that the variable sets of changed and used vars of
+   a program are sensibly defined.
+
+   At most the changed var set is modified. Moreover the behaviour of a program
+   only depends on the vars in the full var set. *)
+
+
+
+(**************************)
+(* Complement of var sets *)
+(**************************)
+
+(* For sets of BIR variables, we need a special complement function. The lookup
+   only considers the name, not the type. So, our special complement should ignore the
+   type as well. *)
+val bir_varset_COMPL_def = Define `bir_varset_COMPL vs =
+  {v | !v'. v' IN vs ==> (bir_var_name v <> bir_var_name v')}`
+
+val IN_bir_varset_COMPL = store_thm ("IN_bir_varset_COMPL",
+``!v vs. v IN bir_varset_COMPL vs <=> (!v'. v' IN vs ==> (bir_var_name v <> bir_var_name v'))``,
+SIMP_TAC std_ss [bir_varset_COMPL_def, GSPECIFICATION]);
+
+val bir_varset_COMPL_EMPTY = store_thm ("bir_varset_COMPL_EMPTY",
+``bir_varset_COMPL EMPTY = UNIV``,
+SIMP_TAC std_ss [EXTENSION, IN_bir_varset_COMPL, NOT_IN_EMPTY, IN_UNIV]);
+
+val bir_varset_COMPL_UNIV = store_thm ("bir_varset_COMPL_UNIV",
+``bir_varset_COMPL UNIV = EMPTY``,
+SIMP_TAC std_ss [EXTENSION, IN_bir_varset_COMPL, NOT_IN_EMPTY, IN_UNIV] >>
+METIS_TAC[]);
+
+val bir_varset_COMPL_SUBSET_COMPL = store_thm ("bir_varset_COMPL_SUBSET_COMPL",
+``!vs. bir_varset_COMPL vs SUBSET COMPL vs``,
+SIMP_TAC std_ss [SUBSET_DEF, IN_bir_varset_COMPL, IN_COMPL] >>
+METIS_TAC[]);
+
+val bir_varset_COMPL_UNION = store_thm ("bir_varset_COMPL_UNION",
+ ``!vs1 vs2. bir_varset_COMPL (vs1 UNION vs2) =
+             bir_varset_COMPL vs1 INTER bir_varset_COMPL vs2``,
+
+SIMP_TAC std_ss [EXTENSION, IN_INTER, IN_UNION, IN_bir_varset_COMPL] >>
+METIS_TAC[])
+
+
+val bir_varset_COMPL_SING = store_thm ("bir_varset_COMPL_SING",
+  ``!v. bir_varset_COMPL {v} = {v' | bir_var_name v' <> bir_var_name v}``,
+SIMP_TAC std_ss [bir_varset_COMPL_def, IN_INSERT, NOT_IN_EMPTY]);
+
+val bir_varset_COMPL_INSERT = store_thm ("bir_varset_COMPL_INSERT",
+ ``!v vs. bir_varset_COMPL (v INSERT vs) =
+          (bir_varset_COMPL vs INTER {v' | bir_var_name v' <> bir_var_name v})``,
+
+SIMP_TAC std_ss [EXTENSION, IN_INTER, IN_bir_varset_COMPL, IN_INSERT,
+  GSPECIFICATION] >>
+METIS_TAC[])
+
+val bir_varset_COMPL_SUBSET = store_thm ("bir_varset_COMPL_SUBSET",
+``!vs1 vs2. vs2 SUBSET vs1 ==> (bir_varset_COMPL vs1 SUBSET bir_varset_COMPL vs2)``,
+SIMP_TAC std_ss [SUBSET_DEF, IN_bir_varset_COMPL]);
+
+
+val bir_varset_COMPL_IN_EVAL = store_thm ("bir_varset_COMPL_IN_EVAL",
+
+``(!v. v IN bir_varset_COMPL EMPTY) /\
+  (!v. ~(v IN bir_varset_COMPL UNIV)) /\
+  (!v vs1 vs2. (v IN bir_varset_COMPL (vs1 UNION vs2)) <=>
+       (v IN bir_varset_COMPL vs1 /\
+        v IN bir_varset_COMPL vs2)) /\
+  (!v vs v'. (v IN bir_varset_COMPL (v' INSERT vs)) <=>
+       (bir_var_name v <> bir_var_name v') /\
+       (v IN bir_varset_COMPL vs))``,
+
+SIMP_TAC std_ss [IN_bir_varset_COMPL, IN_INSERT, IN_UNIV,
+  NOT_IN_EMPTY, IN_UNION, DISJ_IMP_THM, FORALL_AND_THM] >>
+METIS_TAC[]);
+
+
+
+(****************)
+(* Changed vars *)
+(****************)
+
+(* At most the vars in the changed var set are modified *)
+val bir_changed_vars_of_stmtB_THM = store_thm ("bir_changed_vars_of_stmtB_THM",
+``!st stmt.
+   (bir_env_EQ_FOR_VARS (bir_varset_COMPL (bir_changed_vars_of_stmtB stmt))
+        (bir_exec_stmtB_state stmt st).bst_environ (st.bst_environ))``,
+
+Cases_on `stmt` >> (
+  (* Interesting cases are only assign and declare. In all other cases
+     the env is not changed. *)
+  SIMP_TAC std_ss [bir_changed_vars_of_stmtB_def,
+    bir_exec_stmt_assume_SAME_ENV,
+    bir_exec_stmt_assert_SAME_ENV,
+    bir_exec_stmt_observe_SAME_ENV,
+    bir_exec_stmtB_state_def, bir_exec_stmtB_def,
+    bir_env_EQ_FOR_VARS_EQUIV
+  ]
+) >> (
+  SIMP_TAC (std_ss++boolSimps.LIFT_COND_ss) [bir_env_EQ_FOR_VARS_def, bir_varset_COMPL_IN_EVAL]
+) >| [
+  (* declare *)
+  GEN_TAC >>
+  Cases_on `st.bst_environ` >>
+  ASM_SIMP_TAC (std_ss++holBACore_ss) [bir_exec_stmt_declare_def,
+    bir_env_update_def] >>
+  REPEAT CASE_TAC >> (
+    FULL_SIMP_TAC (std_ss++holBACore_ss) [bir_state_set_failed_def,
+      bir_env_lookup_UPDATE]
+  ),
+
+
+  (* assign *)
+  GEN_TAC >>
+  Cases_on `st.bst_environ` >>
+  ASM_SIMP_TAC (std_ss++holBACore_ss) [bir_exec_stmt_assign_def,
+    bir_env_write_def, LET_DEF, bir_env_update_def] >>
+  REPEAT CASE_TAC >> (
+    FULL_SIMP_TAC (std_ss++holBACore_ss) [bir_state_set_failed_def,
+      bir_env_lookup_UPDATE]
+  )
+]);
+
+
+val bir_changed_vars_of_stmt_THM = store_thm ("bir_changed_vars_of_stmt_THM",
+``!st p stmt.
+   (bir_env_EQ_FOR_VARS (bir_varset_COMPL (bir_changed_vars_of_stmt stmt))
+        (bir_exec_stmt_state p stmt st).bst_environ (st.bst_environ))``,
+
+REPEAT GEN_TAC >>
+Cases_on `stmt` >- (
+  SIMP_TAC (std_ss++boolSimps.LIFT_COND_ss++holBACore_ss) [bir_exec_stmt_state_REWRS, LET_THM,
+    bir_changed_vars_of_stmt_def] >>
+  METIS_TAC[bir_changed_vars_of_stmtB_THM]
+) >>
+SIMP_TAC std_ss [bir_exec_stmt_state_REWRS, bir_exec_stmtE_env_unchanged,
+  bir_env_EQ_FOR_VARS_EQUIV]);
+
+
+val bir_changed_vars_of_exec_stmtsB_THM = store_thm ("bir_changed_vars_of_exec_stmtsB_THM",
+``!stmts st ol n.
+   bir_env_EQ_FOR_VARS (bir_varset_COMPL (BIGUNION (IMAGE bir_changed_vars_of_stmtB (set stmts))))
+        (let (ol', n', st') = (bir_exec_stmtsB stmts (ol, n, st)) in
+         st'.bst_environ) (st.bst_environ)``,
+
+Induct >- (
+  SIMP_TAC std_ss [bir_exec_stmtsB_REWRS, LET_THM, bir_env_EQ_FOR_VARS_EQUIV]
+) >>
+REPEAT GEN_TAC >>
+Cases_on `bir_state_is_terminated st` >- (
+  ASM_SIMP_TAC std_ss [bir_exec_stmtsB_REWRS, LET_THM, bir_env_EQ_FOR_VARS_EQUIV]
+) >>
+rename1 `bir_exec_stmtsB (stmt::stmts)` >>
+`?fe st'. bir_exec_stmtB stmt st = (fe, st')` by METIS_TAC[pairTheory.PAIR] >>
+`?ol' n' st''. bir_exec_stmtsB stmts (OPT_CONS fe ol, SUC n, st') =
+               (ol', n', st'')` by METIS_TAC[pairTheory.PAIR] >>
+Q.PAT_X_ASSUM `!st. _` (MP_TAC o Q.SPECL [`st'`, `OPT_CONS fe ol`, `SUC n`]) >>
+MP_TAC (Q.SPECL [`st`, `stmt`] bir_changed_vars_of_stmtB_THM) >>
+ASM_SIMP_TAC list_ss [LET_THM, IMAGE_INSERT, BIGUNION_INSERT, bir_varset_COMPL_UNION,
+  bir_exec_stmtB_state_def, bir_exec_stmtsB_REWRS] >>
+METIS_TAC[INTER_SUBSET, bir_env_EQ_FOR_VARS_SUBSET, bir_env_EQ_FOR_VARS_EQUIV]);
+
+
+val bir_changed_vars_of_block_THM = store_thm ("bir_changed_vars_of_block_THM",
+``!(p:'a bir_program_t) (bl:'a bir_block_t) st.
+   (bir_env_EQ_FOR_VARS (bir_varset_COMPL (bir_changed_vars_of_block bl))
+        (let (ol, n, st') = (bir_exec_block p bl st) in
+         st'.bst_environ) (st.bst_environ))``,
+
+REPEAT STRIP_TAC >>
+`?ol n st'. bir_exec_stmtsB bl.bb_statements ([],0,st) = (ol, n, st')` by
+  METIS_TAC[pairTheory.PAIR] >>
+MP_TAC (Q.SPECL [` bl.bb_statements`, `st`, `[]`, `0`] bir_changed_vars_of_exec_stmtsB_THM) >>
+ASM_SIMP_TAC (std_ss++holBACore_ss++boolSimps.LIFT_COND_ss) [LET_THM, bir_exec_block_def,
+  bir_changed_vars_of_block_def, bir_exec_stmtE_env_unchanged]);
+
+
+val bir_changed_vars_exec_step_THM = store_thm ("bir_changed_vars_exec_step_THM",
+``!(p:'a bir_program_t) st.
+   (bir_env_EQ_FOR_VARS (bir_varset_COMPL (bir_changed_vars_of_program p))
+        ((bir_exec_step_state p st).bst_environ) (st.bst_environ))``,
+
+REPEAT STRIP_TAC >>
+SIMP_TAC (std_ss++boolSimps.LIFT_COND_ss) [bir_exec_step_state_def, bir_exec_step_def,
+  bir_env_EQ_FOR_VARS_EQUIV] >>
+Cases_on ` bir_get_current_statement p st.bst_pc` >- (
+  ASM_SIMP_TAC (std_ss++holBACore_ss) [bir_state_set_failed_def,
+    bir_env_EQ_FOR_VARS_EQUIV]
+) >>
+rename1 `_ = SOME stmt` >>
+ASM_SIMP_TAC std_ss [GSYM bir_exec_stmt_state_def] >>
+DISJ2_TAC >>
+
+`bir_changed_vars_of_stmt stmt SUBSET (bir_changed_vars_of_program p)` by (
+  METIS_TAC[bir_get_current_statement_changed_vars_of]
+) >>
+METIS_TAC[bir_changed_vars_of_stmt_THM, bir_env_EQ_FOR_VARS_SUBSET,
+    bir_varset_COMPL_SUBSET, bir_env_EQ_FOR_VARS_EQUIV]
+);
+
+
+val bir_changed_vars_exec_step_n_THM = store_thm ("bir_changed_vars_exec_step_n_THM",
+``!(p:'a bir_program_t) n st.
+   (bir_env_EQ_FOR_VARS (bir_varset_COMPL (bir_changed_vars_of_program p))
+        ((let (ol, n', st') = bir_exec_step_n p st n in st').bst_environ) (st.bst_environ))``,
+
+GEN_TAC >> Induct >- (
+  SIMP_TAC std_ss [bir_exec_step_n_REWRS, LET_THM, bir_env_EQ_FOR_VARS_EQUIV]
+) >>
+SIMP_TAC (std_ss++boolSimps.LIFT_COND_ss) [bir_exec_step_n_SUC, LET_THM,
+  bir_env_EQ_FOR_VARS_EQUIV] >>
+GEN_TAC >> DISJ2_TAC >>
+Cases_on `bir_exec_step p st` >> rename1 `_ = (fe, st')` >>
+`?l c st''.  (bir_exec_step_n p st' n) = (l, c, st'')` by METIS_TAC[pairTheory.PAIR] >>
+MP_TAC (Q.SPECL [`p`, `st`] bir_changed_vars_exec_step_THM) >>
+Q.PAT_X_ASSUM `!st. _` (MP_TAC o Q.SPEC `st'`) >>
+ASM_SIMP_TAC std_ss [bir_exec_step_state_def, LET_THM] >>
+METIS_TAC[bir_env_EQ_FOR_VARS_EQUIV]);
+
+
+
+
+(************)
+(* All vars *)
+(************)
+
+val bir_state_EQ_FOR_VARS_def = Define `
+  bir_state_EQ_FOR_VARS vs st1 st2 <=> (
+    ?env.
+      (st2 = st1 with bst_environ := env) /\
+      bir_env_EQ_FOR_VARS vs env (st1.bst_environ))`;
+
+val bir_state_EQ_FOR_VARS_ALT_DEF = store_thm ("bir_state_EQ_FOR_VARS_ALT_DEF",
+``!vs st1 st2.
+  bir_state_EQ_FOR_VARS vs st1 st2 <=>
+  (st1.bst_pc = st2.bst_pc) /\ (st1.bst_status = st2.bst_status) /\
+  bir_env_EQ_FOR_VARS vs st1.bst_environ st2.bst_environ``,
+
+SIMP_TAC (std_ss++holBACore_ss++boolSimps.EQUIV_EXTRACT_ss) [bir_state_t_component_equality,
+  bir_state_EQ_FOR_VARS_def, bir_env_EQ_FOR_VARS_EQUIV]);
+
+
+(* At most the vars in the changed var set are modified *)
+val bir_vars_of_stmtB_THM = store_thm ("bir_vars_of_stmtB_THM",
+``!st1 st2 vs stmt.
+    (bir_vars_of_stmtB stmt SUBSET vs) ==>
+    (bir_state_EQ_FOR_VARS vs st1 st2) ==>
+    (let (oo1, st1') = bir_exec_stmtB stmt st1 in
+     let (oo2, st2') = bir_exec_stmtB stmt st2 in
+     ((oo1 = oo2) /\ (bir_state_EQ_FOR_VARS vs st1' st2')))``,
+
+REPEAT STRIP_TAC >>
+FULL_SIMP_TAC std_ss [bir_state_EQ_FOR_VARS_ALT_DEF] >>
+`bir_env_EQ_FOR_VARS (bir_vars_of_stmtB stmt) st1.bst_environ st2.bst_environ` by
+  METIS_TAC[bir_env_EQ_FOR_VARS_SUBSET] >>
+Cases_on `st1.bst_environ` >>
+Cases_on `st2.bst_environ` >>
+rename1 `bir_env_EQ_FOR_VARS _ (BEnv env1) (BEnv env2)` >>
+Cases_on `stmt` >> (
+  FULL_SIMP_TAC std_ss [
+    bir_exec_stmt_assume_SAME_ENV,
+    bir_exec_stmt_assert_SAME_ENV,
+    bir_exec_stmt_observe_SAME_ENV,
+    bir_exec_stmtB_state_def, bir_exec_stmtB_def,
+    bir_env_EQ_FOR_VARS_EQUIV, LET_THM
+  ]
+) >| [
+  (* declare *)
+  FULL_SIMP_TAC (std_ss++holBACore_ss) [bir_exec_stmt_declare_def,
+    bir_env_update_def, bir_vars_of_stmtB_def, SUBSET_DEF, IN_INSERT, NOT_IN_EMPTY,
+    bir_env_EQ_FOR_VARS_def] >>
+  REPEAT CASE_TAC >> (
+    FULL_SIMP_TAC (std_ss++holBACore_ss) [bir_state_set_failed_def,
+      bir_env_lookup_UPDATE, bir_env_varname_is_bound_ALT2_DEF] >>
+    METIS_TAC[optionTheory.option_CLAUSES]
+  ),
+
+  (* assign *)
+  rename1 `bir_exec_stmt_assign v e` >>
+  `bir_eval_exp e (BEnv env1) = bir_eval_exp e (BEnv env2)` by (
+     MATCH_MP_TAC bir_vars_of_exp_THM_EQ_FOR_VARS >>
+     FULL_SIMP_TAC std_ss [bir_env_EQ_FOR_VARS_def, IN_INSERT, bir_vars_of_stmtB_def]
+  ) >>
+  FULL_SIMP_TAC (std_ss++holBACore_ss) [bir_exec_stmt_assign_def,
+    bir_env_write_def, LET_DEF, bir_env_update_def, bir_vars_of_stmtB_def,
+    IN_INSERT, DISJ_IMP_THM, bir_env_EQ_FOR_VARS_def, FORALL_AND_THM,
+    bir_env_check_type_def, bir_env_lookup_type_def] >>
+  REPEAT CASE_TAC >> (
+    FULL_SIMP_TAC (std_ss++holBACore_ss) [bir_state_set_failed_def,
+      bir_env_lookup_UPDATE] >>
+    METIS_TAC[]
+  ),
+
+  (* assert *)
+  rename1 `bir_exec_stmt_assert e` >>
+  `bir_eval_exp e (BEnv env1) = bir_eval_exp e (BEnv env2)` by (
+     MATCH_MP_TAC bir_vars_of_exp_THM_EQ_FOR_VARS >>
+     FULL_SIMP_TAC std_ss [bir_env_EQ_FOR_VARS_def, IN_INSERT, bir_vars_of_stmtB_def]
+  ) >>
+  FULL_SIMP_TAC (std_ss++holBACore_ss) [bir_exec_stmt_assert_def] >>
+  REPEAT CASE_TAC >> (
+    FULL_SIMP_TAC (std_ss++holBACore_ss) [bir_state_set_failed_def]
+  ),
+
+  (* assume *)
+  rename1 `bir_exec_stmt_assume e` >>
+  `bir_eval_exp e (BEnv env1) = bir_eval_exp e (BEnv env2)` by (
+     MATCH_MP_TAC bir_vars_of_exp_THM_EQ_FOR_VARS >>
+     FULL_SIMP_TAC std_ss [bir_env_EQ_FOR_VARS_def, bir_vars_of_stmtB_def]
+  ) >>
+  FULL_SIMP_TAC (std_ss++holBACore_ss) [bir_exec_stmt_assume_def] >>
+  REPEAT CASE_TAC >> (
+    FULL_SIMP_TAC (std_ss++holBACore_ss) [bir_state_set_failed_def]
+  ),
+
+  (* observe *)
+  rename1 `bir_exec_stmt_observe e el fl` >>
+  `!e'. MEM e' (e::el) ==> (bir_eval_exp e' (BEnv env1) = bir_eval_exp e' (BEnv env2))` by (
+     REPEAT STRIP_TAC >>
+     MATCH_MP_TAC bir_vars_of_exp_THM_EQ_FOR_VARS >>
+     FULL_SIMP_TAC std_ss [bir_env_EQ_FOR_VARS_def, bir_vars_of_stmtB_def,
+       IN_BIGUNION, IN_IMAGE, PULL_EXISTS] >>
+     METIS_TAC[]
+  ) >>
+
+  FULL_SIMP_TAC (list_ss++holBACore_ss++pairSimps.gen_beta_ss) [bir_exec_stmt_observe_def,
+    DISJ_IMP_THM, FORALL_AND_THM] >>
+  REPEAT CASE_TAC >> (
+    FULL_SIMP_TAC (std_ss++holBACore_ss) [bir_state_set_failed_def]
+  ) >>
+  `(MAP (\e'. bir_eval_exp e' (BEnv env1)) el) =
+   (MAP (\e'. bir_eval_exp e' (BEnv env2)) el)` suffices_by SIMP_TAC std_ss [] >>
+  ASM_SIMP_TAC std_ss [listTheory.MAP_EQ_f]
+]);
+
+
+val bir_vars_of_stmtB_state_THM = store_thm ("bir_vars_of_stmtB_state_THM",
+``!st1 st2 vs stmt.
+    (bir_vars_of_stmtB stmt SUBSET vs) ==>
+    (bir_state_EQ_FOR_VARS vs st1 st2) ==>
+
+    (bir_state_EQ_FOR_VARS vs
+      (bir_exec_stmtB_state stmt st1)
+      (bir_exec_stmtB_state stmt st2))``,
+
+
+REPEAT STRIP_TAC >>
+MP_TAC (Q.SPECL [`st1`, `st2`, `vs`, `stmt`] bir_vars_of_stmtB_THM) >>
+ASM_SIMP_TAC (std_ss++pairSimps.gen_beta_ss) [LET_DEF,
+  bir_exec_stmtB_state_def]);
+
+
+val bir_vars_of_stmtE_THM = store_thm ("bir_vars_of_stmtE_THM",
+``!st1 st2 vs p stmt.
+    (bir_vars_of_stmtE stmt SUBSET vs) ==>
+    (bir_state_EQ_FOR_VARS vs st1 st2) ==>
+    (bir_state_EQ_FOR_VARS vs
+      (bir_exec_stmtE p stmt st1)
+      (bir_exec_stmtE p stmt st2))``,
+
+REPEAT STRIP_TAC >>
+FULL_SIMP_TAC std_ss [bir_state_EQ_FOR_VARS_ALT_DEF] >>
+`bir_env_EQ_FOR_VARS (bir_vars_of_stmtE stmt) st1.bst_environ st2.bst_environ` by
+  METIS_TAC[bir_env_EQ_FOR_VARS_SUBSET] >>
+Cases_on `stmt` >> (
+  FULL_SIMP_TAC std_ss [bir_vars_of_stmtE_def,
+    bir_exec_stmtE_env_unchanged, bir_exec_stmtE_def]
+) >| [
+  (* Jmp *)
+  rename1 `bir_exec_stmt_jmp _ le _` >>
+  `bir_eval_label_exp le st1.bst_environ = bir_eval_label_exp le st2.bst_environ` by
+    METIS_TAC[bir_vars_of_label_exp_THM_EQ_FOR_VARS] >>
+  FULL_SIMP_TAC std_ss [bir_exec_stmt_jmp_def, bir_state_set_failed_def, bir_exec_stmt_jmp_to_label_def] >>
+  REPEAT CASE_TAC >> ASM_SIMP_TAC (std_ss++holBACore_ss) [],
+
+
+  (* CJmp *)
+  rename1 `bir_exec_stmt_cjmp _ ec le1 le2` >>
+  `(bir_eval_label_exp le1 st1.bst_environ = bir_eval_label_exp le1 st2.bst_environ) /\
+   (bir_eval_label_exp le2 st1.bst_environ = bir_eval_label_exp le2 st2.bst_environ) /\
+   (bir_eval_exp ec st1.bst_environ = bir_eval_exp ec st2.bst_environ)` by
+    METIS_TAC[bir_vars_of_label_exp_THM_EQ_FOR_VARS,
+              bir_vars_of_exp_THM_EQ_FOR_VARS,
+              SUBSET_UNION, bir_env_EQ_FOR_VARS_SUBSET] >>
+
+  FULL_SIMP_TAC std_ss [bir_exec_stmt_cjmp_def, bir_state_set_failed_def,
+     bir_exec_stmt_jmp_to_label_def, bir_exec_stmt_jmp_def] >>
+  REPEAT CASE_TAC >> ASM_SIMP_TAC (std_ss++holBACore_ss) [],
+
+
+  (* Halt *)
+  rename1 `bir_exec_stmt_halt e` >>
+  `bir_eval_exp e st1.bst_environ = bir_eval_exp e st2.bst_environ` by
+    METIS_TAC[bir_vars_of_exp_THM_EQ_FOR_VARS] >>
+  FULL_SIMP_TAC (std_ss++holBACore_ss) [bir_exec_stmt_halt_def]
+]);
+
+
+val bir_vars_of_stmt_THM = store_thm ("bir_vars_of_stmt_THM",
+``!st1 st2 vs p stmt.
+    (bir_vars_of_stmt stmt SUBSET vs) ==>
+    (bir_state_EQ_FOR_VARS vs st1 st2) ==>
+    (let (oo1, st1') = bir_exec_stmt p stmt st1 in
+     let (oo2, st2') = bir_exec_stmt p stmt st2 in
+     ((oo1 = oo2) /\ (bir_state_EQ_FOR_VARS vs st1' st2')))``,
+
+REPEAT STRIP_TAC >>
+Cases_on `stmt` >> (
+  FULL_SIMP_TAC (std_ss++pairSimps.gen_beta_ss++boolSimps.LIFT_COND_ss++
+      bir_TYPES_ss) [
+    bir_vars_of_stmt_def, bir_exec_stmt_state_def,
+    bir_exec_stmt_def, LET_DEF,
+    bir_state_EQ_FOR_VARS_ALT_DEF,
+    bir_program_valid_stateTheory.bir_exec_stmtB_pc_unchanged,
+    bir_state_is_terminated_def]
+) >| [
+  rename1 `bir_vars_of_stmtB stmt` >>
+  MP_TAC (Q.SPECL [`st1`, `st2`, `vs`, `stmt`] bir_vars_of_stmtB_THM) >>
+  FULL_SIMP_TAC (std_ss++pairSimps.gen_beta_ss) [bir_state_EQ_FOR_VARS_ALT_DEF, LET_DEF],
+
+  METIS_TAC[bir_state_EQ_FOR_VARS_ALT_DEF, bir_vars_of_stmtE_THM]
+]);
+
+
+val bir_vars_of_stmt_state_THM = store_thm ("bir_vars_of_stmt_state_THM",
+``!st1 st2 vs p stmt.
+    (bir_vars_of_stmt stmt SUBSET vs) ==>
+    (bir_state_EQ_FOR_VARS vs st1 st2) ==>
+    (bir_state_EQ_FOR_VARS vs
+      (bir_exec_stmt_state p stmt st1)
+      (bir_exec_stmt_state p stmt st2))``,
+
+REPEAT STRIP_TAC >>
+MP_TAC (Q.SPECL [`st1`, `st2`, `vs`, `p`, `stmt`] bir_vars_of_stmt_THM) >>
+ASM_SIMP_TAC (std_ss++pairSimps.gen_beta_ss) [LET_DEF, bir_exec_stmt_state_def]);
+
+
+val bir_vars_of_exec_stmtsB_THM = store_thm ("bir_vars_of_exec_stmtsB_THM",
+``!vs (stmts :'a bir_stmt_basic_t list) st1 st2 l n.
+    (BIGUNION (IMAGE bir_vars_of_stmtB (set stmts)) SUBSET vs) ==>
+    (bir_state_EQ_FOR_VARS vs st1 st2) ==>
+    (let (ol1, n1, st1') = bir_exec_stmtsB stmts (l, n, st1) in
+     let (ol2, n2, st2') = bir_exec_stmtsB stmts (l, n, st2) in
+     ((ol1 = ol2) /\ (n1 = n2) /\ (bir_state_EQ_FOR_VARS vs st1' st2')))``,
+
+GEN_TAC >>
+Induct >- (
+  SIMP_TAC std_ss [bir_exec_stmtsB_REWRS, LET_THM, bir_env_EQ_FOR_VARS_EQUIV]
+) >>
+REPEAT STRIP_TAC >>
+`bir_state_is_terminated st1 = bir_state_is_terminated st2` by
+   FULL_SIMP_TAC std_ss [bir_state_EQ_FOR_VARS_ALT_DEF, bir_state_is_terminated_def] >>
+Cases_on `bir_state_is_terminated st2` >- (
+  FULL_SIMP_TAC std_ss [bir_exec_stmtsB_REWRS, LET_THM, bir_env_EQ_FOR_VARS_EQUIV]
+) >>
+rename1 `bir_exec_stmtsB (stmt::stmts)` >>
+`?fe1 st1'. bir_exec_stmtB stmt st1 = (fe1, st1')` by METIS_TAC[pairTheory.PAIR] >>
+`?fe2 st2'. bir_exec_stmtB stmt st2 = (fe2, st2')` by METIS_TAC[pairTheory.PAIR] >>
+`?ol1 n1 st1''. bir_exec_stmtsB stmts (OPT_CONS fe1 l, SUC n, st1') =
+               (ol1, n1, st1'')` by METIS_TAC[pairTheory.PAIR] >>
+`?ol2 n2 st2''. bir_exec_stmtsB stmts (OPT_CONS fe2 l, SUC n, st2') =
+               (ol2, n2, st2'')` by METIS_TAC[pairTheory.PAIR] >>
+Q.PAT_X_ASSUM `!st. _` (MP_TAC o Q.SPECL [`st1'`, `st2'`, `OPT_CONS fe1 l`, `SUC n`]) >>
+MP_TAC (Q.SPECL [`st1`, `st2`, `vs`, `stmt`] bir_vars_of_stmtB_THM) >>
+FULL_SIMP_TAC list_ss [bir_exec_stmtsB_REWRS, LET_THM,
+  IMAGE_INSERT, BIGUNION_INSERT, UNION_SUBSET] >>
+NTAC 2 STRIP_TAC >>
+REPEAT BasicProvers.VAR_EQ_TAC >>
+FULL_SIMP_TAC std_ss []);
+
+
+
+val bir_vars_of_block_THM = store_thm ("bir_vars_of_block_THM",
+``!(p : 'a bir_program_t) vs (bl :'a bir_block_t) st1 st2.
+    (bir_vars_of_block bl SUBSET vs) ==>
+    (bir_state_EQ_FOR_VARS vs st1 st2) ==>
+    (let (ol1, n1, st1') = bir_exec_block p bl st1 in
+     let (ol2, n2, st2') = bir_exec_block p bl st2 in
+     ((ol1 = ol2) /\ (n1 = n2) /\ (bir_state_EQ_FOR_VARS vs st1' st2')))``,
+
+REPEAT STRIP_TAC >>
+`?ol1 n1 st1'. bir_exec_stmtsB bl.bb_statements ([],0,st1) = (ol1, n1, st1')` by
+  METIS_TAC[pairTheory.PAIR] >>
+`?ol2 n2 st2'. bir_exec_stmtsB bl.bb_statements ([],0,st2) = (ol2, n2, st2')` by
+  METIS_TAC[pairTheory.PAIR] >>
+`(ol1 = ol2) /\ (n1 = n2) /\ bir_state_EQ_FOR_VARS vs st1' st2'` by (
+  MP_TAC (Q.SPECL [`vs`, `bl.bb_statements`, `st1`, `st2`, `[]`, `0`] bir_vars_of_exec_stmtsB_THM) >>
+  FULL_SIMP_TAC std_ss [bir_vars_of_block_def, UNION_SUBSET, LET_THM]
+) >>
+REPEAT BasicProvers.VAR_EQ_TAC >>
+
+MP_TAC (Q.SPECL [`st1'`, `st2'`, `vs`, `p`, `bl.bb_last_statement`] bir_vars_of_stmtE_THM) >>
+FULL_SIMP_TAC (std_ss++boolSimps.LIFT_COND_ss++bir_TYPES_ss) [
+  bir_vars_of_block_def, UNION_SUBSET, LET_THM, bir_exec_block_def,
+  bir_state_EQ_FOR_VARS_ALT_DEF, bir_state_is_terminated_def,
+  bir_program_valid_stateTheory.bir_exec_stmtE_env_unchanged]);
+
+
+val bir_vars_exec_step_THM = store_thm ("bir_vars_exec_step_THM",
+``!p st1 st2 vs.
+    (bir_vars_of_program p SUBSET vs) ==>
+    (bir_state_EQ_FOR_VARS vs st1 st2) ==>
+    (let (oo1, st1') = bir_exec_step p st1 in
+     let (oo2, st2') = bir_exec_step p st2 in
+     ((oo1 = oo2) /\ (bir_state_EQ_FOR_VARS vs st1' st2')))``,
+
+REPEAT STRIP_TAC >>
+`(bir_state_is_terminated st2 = bir_state_is_terminated st1) /\
+ (st1.bst_pc = st2.bst_pc)` by
+  FULL_SIMP_TAC std_ss [bir_state_is_terminated_def, bir_state_EQ_FOR_VARS_ALT_DEF] >>
+ASM_SIMP_TAC (std_ss++boolSimps.LIFT_COND_ss) [bir_exec_step_state_def, bir_exec_step_def,
+  bir_env_EQ_FOR_VARS_EQUIV, LET_THM] >>
+Cases_on ` bir_get_current_statement p st2.bst_pc` >- (
+  FULL_SIMP_TAC (std_ss++holBACore_ss) [bir_state_set_failed_def,
+    bir_state_EQ_FOR_VARS_ALT_DEF,
+    bir_env_EQ_FOR_VARS_EQUIV]
+) >>
+rename1 `_ = SOME stmt` >>
+ASM_SIMP_TAC std_ss [] >>
+DISJ2_TAC >>
+
+`bir_vars_of_stmt stmt SUBSET vs` by (
+  METIS_TAC[bir_get_current_statement_vars_of, SUBSET_TRANS]
+) >>
+
+MP_TAC (Q.SPECL [`st1`, `st2`, `vs`, `p`, `stmt`] bir_vars_of_stmt_THM) >>
+ASM_SIMP_TAC std_ss [LET_THM]);
+
+
+val bir_vars_exec_step_state_THM = store_thm ("bir_vars_exec_step_state_THM",
+``!p st1 st2 vs.
+    (bir_vars_of_program p SUBSET vs) ==>
+    (bir_state_EQ_FOR_VARS vs st1 st2) ==>
+    (bir_state_EQ_FOR_VARS vs (bir_exec_step_state p st1) (bir_exec_step_state p st2))``,
+
+REPEAT STRIP_TAC >>
+MP_TAC (Q.SPECL [`p`, `st1`, `st2`, `vs`] bir_vars_exec_step_THM) >>
+ASM_SIMP_TAC (std_ss++pairSimps.gen_beta_ss) [LET_THM, bir_exec_step_state_def]);
+
+
+
+val bir_vars_exec_infinite_step_fun_THM = store_thm ("bir_vars_exec_infinite_step_fun_THM",
+``!p vs i st1 st2.
+    (bir_vars_of_program p SUBSET vs) ==>
+    (bir_state_EQ_FOR_VARS vs st1 st2) ==>
+    (bir_state_EQ_FOR_VARS vs (bir_exec_infinite_steps_fun p st1 i) (bir_exec_infinite_steps_fun p st2 i))``,
+
+NTAC 2 GEN_TAC >>
+Induct >> (
+  SIMP_TAC std_ss [bir_exec_infinite_steps_fun_REWRS]
+) >>
+METIS_TAC[bir_vars_exec_step_state_THM]);
+
+
+val bir_vars_exec_step_n_THM = store_thm ("bir_vars_exec_step_n_THM",
+``!p vs n st1 st2.
+    (bir_vars_of_program p SUBSET vs) ==>
+    (bir_state_EQ_FOR_VARS vs st1 st2) ==>
+    (let (ol1, n1, st1') = bir_exec_step_n p st1 n in
+     let (ol2, n2, st2') = bir_exec_step_n p st2 n in
+     ((ol1 = ol2) /\ (n1 = n2) /\ (bir_state_EQ_FOR_VARS vs st1' st2')))``,
+
+
+NTAC 2 GEN_TAC >> Induct >- (
+  SIMP_TAC std_ss [bir_exec_step_n_REWRS, LET_THM, bir_env_EQ_FOR_VARS_EQUIV]
+) >>
+REPEAT STRIP_TAC >>
+`?oo1 st1'. bir_exec_step p st1 = (oo1, st1')` by METIS_TAC[pairTheory.PAIR] >>
+`?oo2 st2'. bir_exec_step p st2 = (oo2, st2')` by METIS_TAC[pairTheory.PAIR] >>
+Q.PAT_X_ASSUM `!st1 st2. _` (MP_TAC o Q.SPECL [`st1'`, `st2'`]) >>
+MP_TAC (Q.SPECL [`p`, `st1`, `st2`, `vs`] bir_vars_exec_step_THM) >>
+FULL_SIMP_TAC (std_ss++boolSimps.LIFT_COND_ss++pairSimps.gen_beta_ss) [LET_THM, bir_state_EQ_FOR_VARS_ALT_DEF, bir_state_is_terminated_def,
+  bir_exec_step_n_SUC]);
+
+
+val bir_vars_exec_steps_THM_aux_SOME = prove (
+``!p vs st1 st2 st1' ll c.
+    (bir_vars_of_program p SUBSET vs) ==>
+    (bir_state_EQ_FOR_VARS vs st1 st2) ==>
+    (bir_exec_steps p st1 = (ll, SOME (c, st1'))) ==>
+    (?st2'. (bir_exec_steps p st2 = (ll, SOME (c, st2'))) /\
+            (bir_state_EQ_FOR_VARS vs st1' st2'))``,
+
+REPEAT STRIP_TAC >>
+FULL_SIMP_TAC std_ss [bir_exec_steps_TO_bir_exec_step_n] >>
+`?l1 c1 st2'. bir_exec_step_n p st2 c = (l1, c1, st2')` by METIS_TAC[pairTheory.PAIR] >>
+MP_TAC (Q.SPECL [`p`, `vs`, `c`, `st1`, `st2`] bir_vars_exec_step_n_THM) >>
+FULL_SIMP_TAC std_ss [LET_THM, bir_state_is_terminated_def, bir_state_EQ_FOR_VARS_ALT_DEF] >>
+METIS_TAC[]);
+
+
+
+val bir_vars_exec_steps_THM_aux_NONE = prove (
+``!p vs st1 st2 st1' ll1 ll2.
+    (bir_vars_of_program p SUBSET vs) ==>
+    (bir_state_EQ_FOR_VARS vs st1 st2) ==>
+    (bir_exec_steps p st1 = (ll1, NONE)) ==>
+    (bir_exec_steps p st2 = (ll2, NONE)) ==>
+    (ll1 = ll2)``,
+
+REPEAT STRIP_TAC >>
+FULL_SIMP_TAC std_ss [bir_exec_steps_EQ_NONE,
+  bir_exec_steps_observe_llist_def] >>
+REPEAT BasicProvers.VAR_EQ_TAC >>
+`!i. FST (bir_exec_step p (bir_exec_infinite_steps_fun p st1 i)) =
+     FST (bir_exec_step p (bir_exec_infinite_steps_fun p st2 i))` suffices_by SIMP_TAC std_ss [] >>
+
+GEN_TAC >>
+MP_TAC (Q.SPECL [`p`, `bir_exec_infinite_steps_fun p st1 i`, `bir_exec_infinite_steps_fun p st2 i`, `vs`] bir_vars_exec_step_THM) >>
+MP_TAC (Q.SPECL [`p`, `vs`, `i`, `st1`, `st2`] bir_vars_exec_infinite_step_fun_THM) >>
+ASM_SIMP_TAC (std_ss++pairSimps.gen_beta_ss) [LET_THM]);
+
+
+
+val bir_vars_exec_steps_THM = store_thm ("bir_vars_exec_steps_THM",
+``!p vs st1 st2.
+    (bir_vars_of_program p SUBSET vs) ==>
+    (bir_state_EQ_FOR_VARS vs st1 st2) ==>
+    (let (ll1, res1) = bir_exec_steps p st1 in
+     let (ll2, res2) = bir_exec_steps p st2 in
+     ((ll1 = ll2) /\
+      (case (res1, res2) of
+         | (NONE, NONE) => T
+         | (SOME (n1, st1'), SOME (n2, st2')) =>
+              (n1 = n2) /\ (bir_state_EQ_FOR_VARS vs st1' st2')
+         | (_, _) => F)))``,
+
+REPEAT STRIP_TAC >>
+`?ll1 res1. bir_exec_steps p st1 = (ll1,res1)` by METIS_TAC[pairTheory.PAIR] >>
+`?ll2 res2. bir_exec_steps p st2 = (ll2,res2)` by METIS_TAC[pairTheory.PAIR] >>
+Cases_on `res1` >| [
+  Cases_on `res2` >- (
+    FULL_SIMP_TAC std_ss [LET_THM, pairTheory.pair_case_thm] >>
+    METIS_TAC[bir_vars_exec_steps_THM_aux_NONE]
+  ) >>
+  rename1 `_ = (_, SOME xx)` >> Cases_on `xx` >>
+  rename1 `_ = (_, SOME (c, st2'))` >>
+  MP_TAC (Q.SPECL [`p`, `vs`, `st2`, `st1`] bir_vars_exec_steps_THM_aux_SOME) >>
+  FULL_SIMP_TAC std_ss [bir_state_EQ_FOR_VARS_ALT_DEF, bir_env_EQ_FOR_VARS_EQUIV],
+
+
+  rename1 `_ = (_, SOME xx)` >> Cases_on `xx` >>
+  rename1 `_ = (_, SOME (c, st1'))` >>
+  MP_TAC (Q.SPECL [`p`, `vs`, `st1`, `st2`] bir_vars_exec_steps_THM_aux_SOME) >>
+  ASM_SIMP_TAC std_ss [PULL_EXISTS, LET_THM, pairTheory.pair_case_thm]
+]);
+
+
+
+
+
+val _ = export_theory();
